vp anaphora

Anaphora/Anaphora.v
@@ -1,5 +1,8 @@
+Close Scope nat_scope.
+
 Parameter object : Set.
-Parameter mary : object.
+Parameter MARY : object.
+Parameter JOHN : object.
 
 Inductive Gender : Set :=
     male : Gender
@@ -7,9 +10,19 @@ Inductive Gender : Set :=
 
 Definition Descriptor := Gender.
 
-Definition Env := Descriptor -> object.
+Definition ObjEnv := Descriptor -> object.
+Definition VPEnv := (object -> Prop). (* Just remember the last VP; could be more fine-grained because we have "does", "is", "has" as placehodlers in English.*)
+
+Definition Env : Type := VPEnv * ObjEnv.
 
 Definition Effect := Env -> (Prop * Env).
+Parameter assumedObj : ObjEnv.
+Parameter assumedVP : VPEnv.
+Definition assumed := (assumedVP,assumedObj).
+Definition
+TRUE : Effect -> Set
+     := fun x => let (x',_) := x assumed in x'.
+
 
 Definition S := Effect.
 
@@ -29,25 +42,63 @@ Definition Match : Descriptor -> Descriptor -> bool
     end
   end.
 
-Definition push : Descriptor -> object -> Env -> Env
-:= fun descr obj rho demandedDescr =>
+Definition pushObj : Descriptor -> object -> Env -> Env
+:= fun descr obj env => let (vpEnv, rho) := env in
+     (vpEnv, fun demandedDescr =>
      match Match descr demandedDescr with
        | true => obj
        | false => rho demandedDescr
-     end.
+     end).
 
-Parameter assumed : Env.
+Definition getObj : Env -> Descriptor -> object
+ := fun env descr => let (vpEnv , objEnv) := env in objEnv descr.
+
 
 Definition maryNP : NP
-:= fun vp ρ => vp mary (push female mary ρ).
+:= fun vp ρ => vp MARY (pushObj female MARY ρ).
+
+Definition johnNP : NP
+:= fun vp ρ => vp JOHN (pushObj male JOHN ρ).
 
 Definition sheNP : NP
-:= fun vp ρ => vp (ρ female) ρ.
+:= fun vp ρ => vp (getObj ρ female) ρ.
 
 Definition heNP : NP
-:= fun vp ρ => vp (ρ male) ρ.
+:= fun vp ρ => vp (getObj ρ male) ρ.
+
+
+Definition lift2 : (Prop -> Prop -> Prop) -> Effect -> Effect -> Effect
+:= fun op x y rho1 => let (x' , rho2) := x rho1 in
+                      let (y' , rho3) := y rho2 in
+                       (op x' y' , rho3).
+
+Notation "A [IF] B" := (lift2 (fun x y => y -> x) A B) (at level 9,right associativity).
+
+
+Parameter LEAVE_V : object -> Prop.
+
+
+Definition pureVerb : (object -> Prop) -> VP
+  := fun V x rho => let (vpEnv,objEnv) := rho in (V x, (V,objEnv)).
+
+Definition leavesVP := pureVerb LEAVE_V.
+
+Parameter IS_TIRED : object -> Prop.
+Definition isTiredVP := pureVerb IS_TIRED.
+
+(* EXAMPLE: john leaves if he is tired *)
+Eval cbv in TRUE ((johnNP leavesVP) [IF] (heNP isTiredVP)).
+
+Definition doesTooVP : VP
+   := fun x env => let (vpEnv, objEnv) := env in (vpEnv x,env).
+
+(* EXAMPLE: john leaves if mary does [too] *)
+
+Eval cbv in TRUE ((johnNP leavesVP) [IF] (maryNP doesTooVP)).
+
 
 Parameter attendedTheMeeting : object -> Prop.
+
 Definition attendedTheMeetingVP : VP
   := fun x rho => (attendedTheMeeting x, rho).
 
@@ -58,11 +109,14 @@ Definition IMPLIES : Effect -> Effect -> Effect
 
 Notation "A ==> B" := (IMPLIES A B) (at level 10,right associativity).
 
-Definition
-TRUE : Effect -> Set
-     := fun x => let (x',_) := x assumed in x'.
 
-Theorem thm1 : TRUE (maryNP attendedTheMeetingVP ==> heNP attendedTheMeetingVP).
+
+Theorem thm1 : TRUE (maryNP attendedTheMeetingVP ==> sheNP attendedTheMeetingVP).
 cbv.
 intuition.
 Qed.
+
+Theorem thm2  : TRUE (maryNP attendedTheMeetingVP ==> heNP attendedTheMeetingVP).
+cbv.
+intuition.
+(*False: mary is not male *)
